theories/monotone.v
@@ -1,6 +1,6 @@
 From iris.proofmode Require Import tactics.
 From iris.program_logic Require Export weakestpre.
-From cap_machine Require Export logrel.
+From cap_machine Require Export logrel region_invariants_transitions.
 From iris.base_logic Require Export invariants na_invariants saved_prop.
 Import uPred.
 
@@ -38,9 +38,91 @@ Section monotone.
       + right.
         specialize (Hrelated _ Permanent y HPerm Hy).
         apply std_rel_pub_rtc_Permanent in Hrelated; subst; auto.
+    - destruct Hrelated as [ [Hdom_sta Hrelated] _]. simpl in *.
+      assert (is_Some (W'.1 !! a)) as [y Hy].
+      { apply elem_of_gmap_dom. apply elem_of_subseteq in Hdom_sta. apply Hdom_sta. apply elem_of_gmap_dom.
+        destruct Hstate; eauto. destruct H0;eauto. }
+      destruct Hstate as [Hmono | [Htemp | Hperm] ].
+      + left. specialize (Hrelated _ Monotemporary y Hmono Hy).
+        apply std_rel_pub_rtc_Monotemporary in Hrelated; subst;auto.
+      + right. left.
+        specialize (Hrelated _ Temporary y Htemp Hy).
+        apply std_rel_pub_rtc_Temporary in Hrelated; subst;auto.
+      + right. right.
+        specialize (Hrelated _ Permanent y Hperm Hy).
+        apply std_rel_pub_rtc_Permanent in Hrelated; subst; auto.
   Qed.
 
-  Lemma region_state_nwl_monotone_nl W W' a :
+  Lemma region_state_nwl_monotone_a W W' (a a' : Addr) l :
+    (a <= a')%a →
+    related_sts_a_world W W' a' →
+    region_state_nwl W a l -> region_state_nwl W' a l.
+  Proof.
+    rewrite /region_state_nwl /std.
+    intros Hlt Hrelated Hstate.
+    destruct l.
+    - destruct Hrelated as [ [Hdom_sta Hrelated ] _]. simpl in *.
+      assert (is_Some (W'.1 !! a)) as [y Hy].
+      { apply elem_of_gmap_dom. apply elem_of_subseteq in Hdom_sta. apply Hdom_sta. apply elem_of_gmap_dom;eauto. }
+      specialize (Hrelated a Permanent y Hstate Hy).
+      eapply rtc_implies in Hrelated.
+      apply std_rel_pub_plus_rtc_Permanent in Hrelated; subst; auto.
+      intros r q. destruct (decide (a <= a')%a);auto. 
+    - destruct Hrelated as [ [Hdom_sta Hrelated] _]. simpl in *.
+      assert (is_Some (W'.1 !! a)) as [y Hy].
+      { apply elem_of_gmap_dom. apply elem_of_subseteq in Hdom_sta. apply Hdom_sta. apply elem_of_gmap_dom.
+        destruct Hstate; eauto. }
+      destruct Hstate as [HTemp | HPerm].
+      + left.
+        specialize (Hrelated _ Temporary y HTemp Hy).
+        eapply rtc_implies in Hrelated.
+        apply std_rel_pub_plus_rtc_Temporary in Hrelated; subst;auto.
+        intros r q. destruct (decide (a <= a')%a);auto. 
+      + right.
+        specialize (Hrelated _ Permanent y HPerm Hy).
+        eapply rtc_implies in Hrelated.
+        apply std_rel_pub_plus_rtc_Permanent in Hrelated; subst; auto.
+        intros r q. destruct (decide (a <= a')%a);auto.  
+    - destruct Hrelated as [ [Hdom_sta Hrelated] _]. simpl in *.
+      assert (is_Some (W'.1 !! a)) as [y Hy].
+      { apply elem_of_gmap_dom. apply elem_of_subseteq in Hdom_sta. apply Hdom_sta. apply elem_of_gmap_dom.
+        destruct Hstate; eauto. destruct H0;eauto. }
+      destruct Hstate as [Hmono | [Htemp | Hperm] ].
+      + specialize (Hrelated _ Monotemporary y Hmono Hy).
+        eapply rtc_implies in Hrelated.
+        apply std_rel_pub_rtc_Monotemporary in Hrelated; subst;auto.
+        intros r q. rewrite decide_True;auto.
+      + right. left.
+        specialize (Hrelated _ Temporary y Htemp Hy).
+        eapply rtc_implies in Hrelated.
+        apply std_rel_pub_rtc_Temporary in Hrelated; subst;auto.
+        intros r q. rewrite decide_True;auto.
+      + right. right.
+        specialize (Hrelated _ Permanent y Hperm Hy).
+        eapply rtc_implies in Hrelated.
+        apply std_rel_pub_rtc_Permanent in Hrelated; subst; auto.
+        intros r q. rewrite decide_True;auto.
+  Qed.
+
+  Lemma region_state_nwl_monotone_nm W W' a :
+    related_sts_pub_plus_world W W' →
+    region_state_nwl W a Local -> region_state_nwl W' a Local.
+  Proof.
+    rewrite /region_state_nwl /std.
+    intros Hrelated Hstate.
+    destruct Hrelated as [ [Hdom_sta Hrelated ] _].
+    assert (is_Some (W'.1 !! a)) as [y Hy].
+    { apply elem_of_gmap_dom. apply elem_of_subseteq in Hdom_sta. apply Hdom_sta. apply elem_of_gmap_dom;eauto. destruct Hstate;eauto. }
+    destruct Hstate as [Htemp | Hperm].
+    - left.
+      specialize (Hrelated _ Temporary y Htemp Hy).
+      apply std_rel_pub_plus_rtc_Temporary in Hrelated; subst;auto.
+    - right.
+      specialize (Hrelated _ Permanent y Hperm Hy).
+      apply std_rel_pub_plus_rtc_Permanent in Hrelated; subst; auto.
+  Qed.
+
+  Lemma region_state_nwl_monotone_nm_nl W W' a :
     related_sts_priv_world W W' →
     region_state_nwl W a Global -> region_state_nwl W' a Global.
   Proof.
@@ -53,21 +135,50 @@ Section monotone.
     apply std_rel_rtc_Permanent in Hrelated; subst; auto.
   Qed.
 
-  Lemma region_state_pwl_monotone W W' a :
+  (* Lemma region_state_pwl_monotone W W' a : *)
+  (*   related_sts_pub_plus_world W W' → *)
+  (*   region_state_pwl W a -> region_state_pwl W' a. *)
+  (* Proof. *)
+  (*   rewrite /region_state_pwl /std. *)
+  (*   intros Hrelated Hstate. *)
+  (*   destruct Hrelated as [ [Hdom_sta Hrelated ] _]. simpl in *. *)
+  (*   assert (is_Some (W'.1 !! a)) as [y Hy]. *)
+  (*   { apply elem_of_gmap_dom. apply elem_of_subseteq in Hdom_sta. apply Hdom_sta. apply elem_of_gmap_dom;eauto. } *)
+  (*   specialize (Hrelated _ Temporary y Hstate Hy). *)
+  (*   apply std_rel_pub_plus_rtc_Temporary in Hrelated; subst; auto. *)
+  (* Qed. *)
+
+  Lemma region_state_pwl_monotone_mono W W' a :
     related_sts_pub_world W W' →
-    region_state_pwl W a -> region_state_pwl W' a.
+    region_state_pwl_mono W a -> region_state_pwl_mono W' a.
   Proof.
-    rewrite /region_state_pwl /std.
+    rewrite /region_state_pwl_mono /std.
     intros Hrelated Hstate.
     destruct Hrelated as [ [Hdom_sta Hrelated ] _]. simpl in *.
     assert (is_Some (W'.1 !! a)) as [y Hy].
     { apply elem_of_gmap_dom. apply elem_of_subseteq in Hdom_sta. apply Hdom_sta. apply elem_of_gmap_dom;eauto. }
-    specialize (Hrelated _ Temporary y Hstate Hy).
-    apply std_rel_pub_rtc_Temporary in Hrelated; subst; auto.
+    specialize (Hrelated _ Monotemporary y Hstate Hy).
+    apply std_rel_pub_rtc_Monotemporary in Hrelated; subst; auto.
+  Qed.
+
+  Lemma region_state_pwl_monotone_a W W' a a' :
+    (a <= a')%a →
+    related_sts_a_world W W' a' →
+    region_state_pwl_mono W a -> region_state_pwl_mono W' a.
+  Proof.
+    rewrite /region_state_pwl_mono /std.
+    intros Hle Hrelated Hstate.
+    destruct Hrelated as [ [Hdom_sta Hrelated ] _]. simpl in *.
+    assert (is_Some (W'.1 !! a)) as [y Hy].
+    { apply elem_of_gmap_dom. apply elem_of_subseteq in Hdom_sta. apply Hdom_sta. apply elem_of_gmap_dom;eauto. }
+    specialize (Hrelated _ Monotemporary y Hstate Hy).
+    eapply rtc_implies in Hrelated. 
+    apply std_rel_pub_rtc_Monotemporary in Hrelated; subst; auto.
+    intros r q. rewrite decide_True;auto. 
   Qed.
 
   Lemma region_state_U_monotone W W' a :
-    related_sts_pub_world W W' →
+    related_sts_pub_plus_world W W' →
     region_state_U W a -> region_state_U W' a.
   Proof.
     rewrite /region_state_U /std.
@@ -80,16 +191,61 @@ Section monotone.
     destruct Hstate as [Hstate|[Hstate|[w Hstate] ] ].
     - specialize (Hrelated _ Temporary y Hstate Hy).
       destruct (decide (y = Temporary)); subst; auto.
-      apply std_rel_pub_rtc_Temporary in Hrelated; auto. contradiction.
+      apply std_rel_pub_plus_rtc_Temporary in Hrelated; auto. contradiction.
     - specialize (Hrelated _ Permanent y Hstate Hy).
-      apply std_rel_pub_rtc_Permanent in Hrelated; auto. subst y; auto.
+      apply std_rel_pub_plus_rtc_Permanent in Hrelated; auto. subst y; auto.
     - specialize (Hrelated _ (Static {[a:=w]}) y Hstate Hy).
-      eapply std_rel_pub_rtc_Static in Hrelated; eauto. destruct Hrelated; subst y; eauto.
+      eapply std_rel_pub_plus_rtc_Static in Hrelated; eauto. destruct Hrelated; subst y; eauto.
   Qed.
 
-  Lemma region_state_U_pwl_monotone W W' a :
+  Lemma region_state_U_monotone_mono W W' a :
+    related_sts_pub_plus_world W W' →
+    region_state_U_mono W a -> region_state_U_mono W' a.
+  Proof.
+    rewrite /region_state_U_mono /std.
+    intros Hrelated Hstate.
+    destruct Hrelated as [ [Hdom_sta Hrelated ] _]. simpl in *.
+    assert (is_Some (W'.1 !! a)) as [y Hy].
+    { apply elem_of_gmap_dom. apply elem_of_subseteq in Hdom_sta. apply Hdom_sta. apply elem_of_gmap_dom;eauto.
+      destruct Hstate as [Hstate | [Hstate | [Hstate | [ [w state] |  [w Hstate] ] ] ] ];eauto. }
+    destruct Hstate as [Hstate | [Hstate | [Hstate | [ [w Hstate] |  [w Hstate] ] ] ] ].
+    - specialize (Hrelated _ _ y Hstate Hy).
+      apply std_rel_pub_plus_rtc_Monotemporary in Hrelated;eauto.
+      destruct Hrelated as [-> | [? ->] ];subst;rewrite Hy;eauto. repeat right. eauto. 
+    - specialize (Hrelated _ Temporary y Hstate Hy).
+      destruct (decide (y = Temporary)); subst; auto.
+      apply std_rel_pub_plus_rtc_Temporary in Hrelated; auto. contradiction.
+    - specialize (Hrelated _ Permanent y Hstate Hy).
+      apply std_rel_pub_plus_rtc_Permanent in Hrelated; auto. subst y; auto.
+    - specialize (Hrelated _ (Static {[a:=w]}) y Hstate Hy).
+      eapply std_rel_pub_plus_rtc_Static in Hrelated; eauto. destruct Hrelated; subst y; eauto.
+      right;right;right;left. eauto. 
+    - specialize (Hrelated _ _ y Hstate Hy).
+      eapply std_rel_pub_plus_rtc_Uninitialized in Hrelated; eauto.
+      destruct Hrelated as [-> | [? ->] ]; eauto. repeat right;eauto. 
+  Qed.
+
+  (* Lemma region_state_U_pwl_monotone W W' a : *)
+  (*   related_sts_pub_plus_world W W' → *)
+  (*   region_state_U_pwl W a -> region_state_U_pwl W' a. *)
+  (* Proof. *)
+  (*   rewrite /region_state_U /std. *)
+  (*   intros Hrelated Hstate. *)
+  (*   destruct Hrelated as [ [Hdom_sta Hrelated ] _]. simpl in *. *)
+  (*   assert (is_Some (W'.1 !! a)) as [y Hy]. *)
+  (*   { apply elem_of_gmap_dom. apply elem_of_subseteq in Hdom_sta. apply Hdom_sta. apply elem_of_gmap_dom;eauto. *)
+  (*     destruct Hstate as [? | [? ?] ]; eauto. } *)
+  (*   destruct Hstate as [Hstate|[? Hstate] ]. *)
+  (*   - specialize (Hrelated _ Temporary y Hstate Hy). *)
+  (*     destruct (decide (y = Temporary)); subst; left; auto. *)
+  (*     apply std_rel_pub_plus_rtc_Temporary in Hrelated; auto. contradiction. *)
+  (*   - specialize (Hrelated _ (Static {[a:=x]}) y Hstate Hy). *)
+  (*     eapply std_rel_pub_plus_rtc_Static in Hrelated; eauto. destruct Hrelated; subst y; [left | right]; eauto. *)
+  (* Qed. *)
+
+  Lemma region_state_U_pwl_monotone_mono W W' a :
     related_sts_pub_world W W' →
-    region_state_U_pwl W a -> region_state_U_pwl W' a.
+    region_state_U_pwl_mono W a -> region_state_U_pwl_mono W' a.
   Proof.
     rewrite /region_state_U /std.
     intros Hrelated Hstate.
@@ -98,11 +254,37 @@ Section monotone.
     { apply elem_of_gmap_dom. apply elem_of_subseteq in Hdom_sta. apply Hdom_sta. apply elem_of_gmap_dom;eauto.
       destruct Hstate as [? | [? ?] ]; eauto. }
     destruct Hstate as [Hstate|[? Hstate] ].
-    - specialize (Hrelated _ Temporary y Hstate Hy).
-      destruct (decide (y = Temporary)); subst; left; auto.
-      apply std_rel_pub_rtc_Temporary in Hrelated; auto. contradiction.
-    - specialize (Hrelated _ (Static {[a:=x]}) y Hstate Hy).
-      eapply std_rel_pub_rtc_Static in Hrelated; eauto. destruct Hrelated; subst y; [left | right]; eauto.
+    - specialize (Hrelated _ Monotemporary y Hstate Hy).
+      destruct (decide (y = Monotemporary)); subst; left; auto.
+      apply std_rel_pub_rtc_Monotemporary in Hrelated; auto. contradiction.
+    - specialize (Hrelated _ (Uninitialized x) y Hstate Hy).
+      eapply std_rel_pub_rtc_Uninitialized in Hrelated; eauto. destruct Hrelated;subst y; [left | right]; eauto.
+  Qed.
+
+  Lemma region_state_U_pwl_monotone_mono_a W W' a a' :
+    related_sts_a_world W W' a' →
+    region_state_U_pwl_mono W a -> region_state_U_pwl_mono W' a.
+  Proof.
+    rewrite /region_state_U /std.
+    intros Hrelated Hstate.
+    destruct Hrelated as [ [Hdom_sta Hrelated ] _]. simpl in *.
+    assert (is_Some (W'.1 !! a)) as [y Hy].
+    { apply elem_of_gmap_dom. apply elem_of_subseteq in Hdom_sta. apply Hdom_sta. apply elem_of_gmap_dom;eauto.
+      destruct Hstate as [? | [? ?] ]; eauto. }
+    destruct Hstate as [Hstate|[? Hstate] ].
+    - specialize (Hrelated _ Monotemporary y Hstate Hy).
+      destruct (decide (y = Monotemporary)); subst; auto. left;auto. 
+      destruct (decide (a <= a')%a). 
+      + apply std_rel_pub_rtc_Monotemporary in Hrelated; subst;auto. contradiction.
+      + apply std_rel_pub_plus_rtc_Monotemporary in Hrelated; subst;auto. 
+        destruct Hrelated as [-> | [? ->] ];
+        rewrite /region_state_U_pwl_mono;eauto.
+    - specialize (Hrelated _ (Uninitialized x) y Hstate Hy).
+      destruct (decide (a <= a')%a). 
+      + eapply std_rel_pub_rtc_Uninitialized in Hrelated; eauto.
+        destruct Hrelated; subst y; [left | right]; eauto.
+      + eapply std_rel_pub_plus_rtc_Uninitialized in Hrelated; eauto.
+        destruct Hrelated as [Hy' | [w' Hy'] ]; subst y; [left | right]; eauto.
   Qed.
 
   (* The following lemma is not required for monotonicity, but is interesting for use in examples *)
@@ -123,16 +305,18 @@ Section monotone.
     related_sts_pub_world W W' →
     (std W) !! a = Some Revoked ->
     (std W') !! a = Some Revoked ∨
-    (std W') !! a = Some Temporary.
+    (std W') !! a = Some Temporary ∨
+    (std W') !! a = Some Monotemporary ∨
+    (std W') !! a = Some Permanent.
   Proof.
-    rewrite /region_state_pwl /std.
+    rewrite /region_state_pwl_mono /std.
     intros Hrelated Hstate.
     destruct Hrelated as [ [Hdom_sta Hrelated ] _]. simpl in *.
     assert (is_Some (W'.1 !! a)) as [y Hy].
     { apply elem_of_gmap_dom. apply elem_of_subseteq in Hdom_sta. apply Hdom_sta. apply elem_of_gmap_dom;eauto. }
     specialize (Hrelated _ Revoked y Hstate Hy).
     apply std_rel_pub_rtc_Revoked in Hrelated; auto.
-    destruct Hrelated as [Htemp | Hrev]; subst; auto.
+    destruct Hrelated as [Htemp | [Hperm | [Hmono | Hrev] ] ]; subst; auto.
   Qed.
 
   Lemma interp_monotone W W' w :
@@ -161,7 +345,8 @@ Section monotone.
       iDestruct "Hw" as (p Hfl) "#[Hrw Hrel]".
       iExists _. iSplit;eauto. iFrame "#".
       iDestruct "Hrel" as %Hrel.
-      iPureIntro. apply region_state_pwl_monotone with W;auto.
+      iPureIntro.
+      apply region_state_pwl_monotone_mono with W;auto.
     - iApply (big_sepL_mono with "Hw").
       iIntros (n y Hsome) "Hw".
       iDestruct "Hw" as (p Hfl) "#[Hrw Hrel]".
@@ -171,13 +356,18 @@ Section monotone.
     - iModIntro. iIntros (r W'').
       destruct l; simpl.
       + iIntros (Hrelated').
-        iAssert (future_world Global W W'')%I as "Hrelated".
+        iAssert (future_world Global a W W'')%I as "Hrelated".
         { iPureIntro. apply related_sts_pub_priv_trans_world with W'; auto. }
         iSpecialize ("Hw" $! r W'' with "Hrelated").
         iApply "Hw".
       + iIntros (Hrelated').
-        iAssert (future_world Local W W'')%I as "Hrelated".
-        { iPureIntro. apply related_sts_pub_trans_world with W'; auto. }
+        iAssert (future_world Local a W W'')%I as "Hrelated".
+        { iPureIntro. apply related_sts_pub_pub_plus_trans_world with W'; auto. }
+        iSpecialize ("Hw" $! r W'' with "Hrelated").
+        iApply "Hw".
+      + iIntros (Hrelated').
+        iAssert (future_world Monotone a0 W W'')%I as "Hrelated".
+        { iPureIntro. apply related_sts_pub_a_trans_world with W'; auto. }
         iSpecialize ("Hw" $! r W'' with "Hrelated").
         iApply "Hw".
     - iApply (big_sepL_mono with "Hw").
@@ -192,7 +382,7 @@ Section monotone.
       iDestruct "Hw" as (p Hfl) "#[Hrw Hrel]".
       iExists _. iSplit;eauto. iFrame "#".
       iDestruct "Hrel" as %Hrel.
-      iPureIntro. apply region_state_pwl_monotone with W;auto.
+      iPureIntro. apply region_state_pwl_monotone_mono with W;auto.
     - destruct l; simpl.
       + iApply (big_sepL_mono with "Hw").
         iIntros (n y Hsome) "Hw".
@@ -215,6 +405,23 @@ Section monotone.
           iDestruct "Hst" as %Hst.
           iPureIntro.
           eapply region_state_U_monotone; eauto.
+          apply related_sts_pub_pub_plus_world;auto.
+      + iDestruct "Hw" as "[Hw1 Hw2]".
+        iSplitL "Hw1".
+        * iApply (big_sepL_mono with "Hw1").
+          iIntros (n y Hsome) "Hw".
+          iDestruct "Hw" as (p Hfl) "#[Hrw Hst ]".
+          iExists _. iSplit;eauto. iFrame "#".
+          iDestruct "Hst" as %Hstd.
+          iPureIntro. eapply (region_state_nwl_monotone W W' _ Monotone); auto.
+        * iApply (big_sepL_mono with "Hw2").
+          iIntros (n y Hsome) "Hw".
+          iDestruct "Hw" as (p Hfl) "#[Hrw Hst ]".
+          iExists _. iSplit;eauto. iFrame "#".
+          iDestruct "Hst" as %Hst.
+          iPureIntro.
+          eapply region_state_U_monotone_mono; eauto.
+          apply related_sts_pub_pub_plus_world;auto. 
     - destruct l; auto.
       iDestruct "Hw" as "[Hbe Hexec]".
       iSplit.
@@ -223,13 +430,13 @@ Section monotone.
         iDestruct "Hw" as (p Hfl) "#[Hrw Hrel ]".
         iExists _. iSplit;eauto. iFrame "#".
         iDestruct "Hrel" as %Hrel.
-        iPureIntro. apply region_state_pwl_monotone with W;auto. }
+        iPureIntro. apply region_state_pwl_monotone_mono with W;auto. }
       { iApply (big_sepL_mono with "Hexec").
         iIntros (n y Hsome) "Hw".
         iDestruct "Hw" as (p Hfl) "#[Hrw Hrel ]".
         iExists _. iSplit;eauto. iFrame "#".
         iDestruct "Hrel" as %Hrel.
-        iPureIntro. apply region_state_U_pwl_monotone with W;auto. }
+        iPureIntro. apply region_state_U_pwl_monotone_mono with W;auto. }
     - destruct l; simpl.
       + iApply (big_sepL_mono with "Hw").
         iIntros (n y Hsome) "Hw".
@@ -252,6 +459,23 @@ Section monotone.
           iDestruct "Hst" as %Hst.
           iPureIntro.
           eapply region_state_U_monotone; eauto.
+          apply related_sts_pub_pub_plus_world;auto.
+      + iDestruct "Hw" as "[Hw1 Hw2]".
+        iSplitL "Hw1".
+        * iApply (big_sepL_mono with "Hw1").
+          iIntros (n y Hsome) "Hw".
+          iDestruct "Hw" as (p Hfl) "#[Hrw Hst ]".
+          iExists _. iSplit;eauto. iFrame "#".
+          iDestruct "Hst" as %Hstd.
+          iPureIntro. eapply (region_state_nwl_monotone W W' _ Monotone); auto.
+        * iApply (big_sepL_mono with "Hw2").
+          iIntros (n y Hsome) "Hw".
+          iDestruct "Hw" as (p Hfl) "#[Hrw Hst ]".
+          iExists _. iSplit;eauto. iFrame "#".
+          iDestruct "Hst" as %Hst.
+          iPureIntro.
+          eapply region_state_U_monotone_mono; eauto.
+          apply related_sts_pub_pub_plus_world;auto.
     - destruct l; auto.
       iDestruct "Hw" as "[Hbe Hexec]".
       iSplit.
@@ -260,16 +484,337 @@ Section monotone.
         iDestruct "Hw" as (p Hfl) "#[Hrw Hrel ]".
         iExists _. iSplit;eauto. iFrame "#".
         iDestruct "Hrel" as %Hrel.
-        iPureIntro. apply region_state_pwl_monotone with W;auto. }
+        iPureIntro. apply region_state_pwl_monotone_mono with W;auto. }
       { iApply (big_sepL_mono with "Hexec").
         iIntros (n y Hsome) "Hw".
         iDestruct "Hw" as (p Hfl) "#[Hrw Hrel ]".
         iExists _. iSplit;eauto. iFrame "#".
         iDestruct "Hrel" as %Hrel.
-        iPureIntro. apply region_state_U_pwl_monotone with W;auto. }
+        iPureIntro. apply region_state_U_pwl_monotone_mono with W;auto. }
   Qed.
 
-  Lemma interp_monotone_nl W W' w :
+  Definition aOf (w : Word) : Addr :=
+    match w with
+    | inl _ => addr_reg.top
+    | inr (p,_,_,e,a) => if isU p then a else e
+    end.
+
+  Lemma region_addrs_lookup_le b e a n :
+    region_addrs b e !! n = Some a →
+    (a <= e)%a.
+  Proof.
+    intros Hlookup.
+    assert (a ∈ (region_addrs b e)) as Hin.
+    { apply elem_of_list_lookup. eauto. }
+    apply elem_of_region_addrs in Hin as [? ?].
+    solve_addr.
+  Qed. 
+
+  Lemma interp_monotone_a W W' w :
+    ⌜related_sts_a_world W W' (aOf w)⌝ -∗
+    interp W w -∗ interp W' w.
+  Proof.
+    iIntros (Hrelated) "#Hw".
+    rewrite /interp /= fixpoint_interp1_eq /=.
+    destruct w; rewrite fixpoint_interp1_eq /=; auto.
+    destruct c,p,p,p,p; auto; simpl in Hrelated.
+    - iApply (big_sepL_mono with "Hw").
+      iIntros (n y Hsome) "Hw".
+      iDestruct "Hw" as (p Hfl) "#[Hrw Hrel]".
+      iExists _. iSplit;eauto. iFrame "#".
+      iDestruct "Hrel" as %Hrel.
+      iPureIntro. apply region_state_nwl_monotone_a with W a0;auto.
+      eapply region_addrs_lookup_le;eauto. 
+    - iApply (big_sepL_mono with "Hw").
+      iIntros (n y Hsome) "Hw".
+      iDestruct "Hw" as (p Hfl) "#[Hrw Hrel]".
+      iExists _. iSplit;eauto. iFrame "#".
+      iDestruct "Hrel" as %Hrel.
+      iPureIntro. apply region_state_nwl_monotone_a with W a0;auto. eapply region_addrs_lookup_le;eauto. 
+    - destruct l; auto.
+      iApply (big_sepL_mono with "Hw").
+      iIntros (n y Hsome) "Hw".
+      iDestruct "Hw" as (p Hfl) "#[Hrw Hrel]".
+      iExists _. iSplit;eauto. iFrame "#".
+      iDestruct "Hrel" as %Hrel.
+      iPureIntro.
+      apply region_state_pwl_monotone_a with W a0;auto. eapply region_addrs_lookup_le;eauto. 
+    - iApply (big_sepL_mono with "Hw").
+      iIntros (n y Hsome) "Hw".
+      iDestruct "Hw" as (p Hfl) "#[Hrw Hrel]".
+      iExists _. iSplit;eauto. iFrame "#".
+      iDestruct "Hrel" as %Hrel.
+      iPureIntro. apply region_state_nwl_monotone_a with W a0;auto. eapply region_addrs_lookup_le;eauto. 
+    - iModIntro. iIntros (r W'').
+      destruct l; simpl.
+      + iIntros (Hrelated').
+        iAssert (future_world Global a W W'')%I as "Hrelated".
+        { iPureIntro. apply related_sts_a_priv_trans_world with W' a0; auto. }
+        iSpecialize ("Hw" $! r W'' with "Hrelated").
+        iApply "Hw".
+      + iIntros (Hrelated').
+        iAssert (future_world Local a W W'')%I as "Hrelated".
+        { iPureIntro. apply related_sts_a_pub_plus_trans_world with W' a0; auto. }
+        iSpecialize ("Hw" $! r W'' with "Hrelated").
+        iApply "Hw".
+      + iIntros (Hrelated').
+        iAssert (future_world Monotone a0 W W'')%I as "Hrelated".
+        { iPureIntro. apply related_sts_a_trans_world with W';auto. }
+        iSpecialize ("Hw" $! r W'' with "Hrelated").
+        iApply "Hw".
+    - iApply (big_sepL_mono with "Hw").
+      iIntros (n y Hsome) "Hw".
+      iDestruct "Hw" as (p Hfl) "#[Hrw Hrel]".
+      iExists _. iSplit;eauto. iFrame "#".
+      iDestruct "Hrel" as %Hrel.
+      iPureIntro. apply region_state_nwl_monotone_a with W a0;auto. eapply region_addrs_lookup_le;eauto. 
+    - destruct l; auto.
+      iApply (big_sepL_mono with "Hw").
+      iIntros (n y Hsome) "Hw".
+      iDestruct "Hw" as (p Hfl) "#[Hrw Hrel]".
+      iExists _. iSplit;eauto. iFrame "#".
+      iDestruct "Hrel" as %Hrel.
+      iPureIntro. apply region_state_pwl_monotone_a with W a0;auto. eapply region_addrs_lookup_le;eauto. 
+    - destruct l; simpl.
+      + iApply (big_sepL_mono with "Hw").
+        iIntros (n y Hsome) "Hw".
+        iDestruct "Hw" as (p Hfl) "#[Hrw Hst]".
+        iExists _. iSplit;eauto. iFrame "#".
+        iDestruct "Hst" as %Hst.
+        iPureIntro. apply region_state_nwl_monotone_nm_nl with W;auto.
+        apply related_sts_pub_plus_priv_world, related_sts_a_pub_plus_world with a;auto. 
+      + iDestruct "Hw" as "[Hw1 Hw2]".
+        iSplitL "Hw1".
+        * iApply (big_sepL_mono with "Hw1").
+          iIntros (n y Hsome) "Hw".
+          iDestruct "Hw" as (p Hfl) "#[Hrw Hst ]".
+          iExists _. iSplit;eauto. iFrame "#".
+          iDestruct "Hst" as %Hstd.
+          iPureIntro. eapply (region_state_nwl_monotone_a W W' _ (addr_reg.min a a0) Local); auto.
+          eapply region_addrs_lookup_le;eauto.  apply related_sts_a_weak_world with a;auto. solve_addr. 
+        * iApply (big_sepL_mono with "Hw2").
+          iIntros (n y Hsome) "Hw".
+          iDestruct "Hw" as (p Hfl) "#[Hrw Hst ]".
+          iExists _. iSplit;eauto. iFrame "#".
+          iDestruct "Hst" as %Hst.
+          iPureIntro.
+          eapply region_state_U_monotone; eauto.
+          apply related_sts_a_pub_plus_world with a;auto.
+      + iDestruct "Hw" as "[Hw1 Hw2]".
+        iSplitL "Hw1".
+        * iApply (big_sepL_mono with "Hw1").
+          iIntros (n y Hsome) "Hw".
+          iDestruct "Hw" as (p Hfl) "#[Hrw Hst ]".
+          iExists _. iSplit;eauto. iFrame "#".
+          iDestruct "Hst" as %Hstd.
+          iPureIntro. eapply (region_state_nwl_monotone_a W W' _ (addr_reg.min a a0) Monotone); auto.
+          eapply region_addrs_lookup_le;eauto.  apply related_sts_a_weak_world with a;auto. solve_addr.
+        * iApply (big_sepL_mono with "Hw2").
+          iIntros (n y Hsome) "Hw".
+          iDestruct "Hw" as (p Hfl) "#[Hrw Hst ]".
+          iExists _. iSplit;eauto. iFrame "#".
+          iDestruct "Hst" as %Hst.
+          iPureIntro.
+          eapply region_state_U_monotone_mono; eauto.
+          apply related_sts_a_pub_plus_world with a;auto.
+    - destruct l; auto.
+      iDestruct "Hw" as "[Hbe Hexec]".
+      iSplit.
+      { iApply (big_sepL_mono with "Hbe").
+        iIntros (n y Hsome) "Hw".
+        iDestruct "Hw" as (p Hfl) "#[Hrw Hrel ]".
+        iExists _. iSplit;eauto. iFrame "#".
+        iDestruct "Hrel" as %Hrel.
+        iPureIntro. apply region_state_pwl_monotone_a with W (addr_reg.min a a0);auto.
+        eapply region_addrs_lookup_le;eauto. apply related_sts_a_weak_world with a;auto. solve_addr.
+      }
+      { iApply (big_sepL_mono with "Hexec").
+        iIntros (n y Hsome) "Hw".
+        iDestruct "Hw" as (p Hfl) "#[Hrw Hrel ]".
+        iExists _. iSplit;eauto. iFrame "#".
+        iDestruct "Hrel" as %Hrel.
+        iPureIntro. apply region_state_U_pwl_monotone_mono_a with W (addr_reg.min a a0);auto.
+        apply related_sts_a_weak_world with a;auto. solve_addr. }
+    - destruct l; simpl.
+      + iApply (big_sepL_mono with "Hw").
+        iIntros (n y Hsome) "Hw".
+        iDestruct "Hw" as (p Hfl) "#[Hrw Hst ]".
+        iExists _. iSplit;eauto. iFrame "#".
+        iDestruct "Hst" as %Hst.
+        iPureIntro. apply region_state_nwl_monotone_nm_nl with W;auto.
+        apply related_sts_pub_plus_priv_world, related_sts_a_pub_plus_world with a;auto.
+      + iDestruct "Hw" as "[Hw1 Hw2]".
+        iSplitL "Hw1".
+        * iApply (big_sepL_mono with "Hw1").
+          iIntros (n y Hsome) "Hw".
+          iDestruct "Hw" as (p Hfl) "#[Hrw Hst ]".
+          iExists _. iSplit;eauto. iFrame "#".
+          iDestruct "Hst" as %Hstd.
+          iPureIntro. eapply (region_state_nwl_monotone_a W W' _ (addr_reg.min a a0) Local); auto.
+          eapply region_addrs_lookup_le;eauto. apply related_sts_a_weak_world with a;auto. solve_addr.
+        * iApply (big_sepL_mono with "Hw2").
+          iIntros (n y Hsome) "Hw".
+          iDestruct "Hw" as (p Hfl) "#[Hrw Hst ]".
+          iExists _. iSplit;eauto. iFrame "#".
+          iDestruct "Hst" as %Hst.
+          iPureIntro.
+          eapply region_state_U_monotone; eauto.
+          apply related_sts_a_pub_plus_world with a;auto.
+      + iDestruct "Hw" as "[Hw1 Hw2]".
+        iSplitL "Hw1".
+        * iApply (big_sepL_mono with "Hw1").
+          iIntros (n y Hsome) "Hw".
+          iDestruct "Hw" as (p Hfl) "#[Hrw Hst ]".
+          iExists _. iSplit;eauto. iFrame "#".
+          iDestruct "Hst" as %Hstd.
+          iPureIntro. eapply (region_state_nwl_monotone_a W W' _ (addr_reg.min a a0)  Monotone); auto.
+          eapply region_addrs_lookup_le;eauto. apply related_sts_a_weak_world with a;auto. solve_addr.
+         * iApply (big_sepL_mono with "Hw2").
+          iIntros (n y Hsome) "Hw".
+          iDestruct "Hw" as (p Hfl) "#[Hrw Hst ]".
+          iExists _. iSplit;eauto. iFrame "#".
+          iDestruct "Hst" as %Hst.
+          iPureIntro.
+          eapply region_state_U_monotone_mono; eauto.
+          apply related_sts_a_pub_plus_world with a;auto.
+    - destruct l; auto.
+      iDestruct "Hw" as "[Hbe Hexec]".
+      iSplit.
+      { iApply (big_sepL_mono with "Hbe").
+        iIntros (n y Hsome) "Hw".
+        iDestruct "Hw" as (p Hfl) "#[Hrw Hrel ]".
+        iExists _. iSplit;eauto. iFrame "#".
+        iDestruct "Hrel" as %Hrel.
+        iPureIntro. apply region_state_pwl_monotone_a with W (addr_reg.min a a0);auto.
+        eapply region_addrs_lookup_le;eauto. apply related_sts_a_weak_world with a;auto. solve_addr.
+      }
+      { iApply (big_sepL_mono with "Hexec").
+        iIntros (n y Hsome) "Hw".
+        iDestruct "Hw" as (p Hfl) "#[Hrw Hrel ]".
+        iExists _. iSplit;eauto. iFrame "#".
+        iDestruct "Hrel" as %Hrel.
+        iPureIntro. apply region_state_U_pwl_monotone_mono_a with W a;auto. }
+  Qed.
+
+  Definition isMonotoneWord (w : Word) :=
+    match w with
+    | inl _ => false
+    | inr (_,l,_,_,_) => isMonotone l
+    end.
+
+  Lemma interp_monotone_nm W W' w :
+    ⌜related_sts_pub_plus_world W W'⌝ -∗ ⌜isMonotoneWord w = false⌝ -∗
+    interp W w -∗ interp W' w.
+  Proof.
+    iIntros (Hrelated Hnl) "#Hw".
+    rewrite /interp /= fixpoint_interp1_eq /=.
+    destruct w; rewrite fixpoint_interp1_eq /=; auto.
+    destruct c,p,p,p,p; auto.
+    - iApply (big_sepL_mono with "Hw").
+      iIntros (n y Hsome) "Hw".
+      iDestruct "Hw" as (p Hfl) "#[Hrw Hrel ]".
+      iExists _. iSplit;eauto. iFrame "#".
+      iDestruct "Hrel" as %Hrel.
+      iPureIntro. destruct l; try discriminate.
+      apply region_state_nwl_monotone_nm_nl with W;auto.
+      apply related_sts_pub_plus_priv_world;auto.
+      apply region_state_nwl_monotone_nm with W;auto.
+    - iApply (big_sepL_mono with "Hw").
+      iIntros (n y Hsome) "Hw".
+      iDestruct "Hw" as (p Hfl) "#[Hrw Hrel ]".
+      iExists _. iSplit;eauto. iFrame "#".
+      iDestruct "Hrel" as %Hrel.
+      iPureIntro. destruct l; try discriminate.
+      apply region_state_nwl_monotone_nm_nl with W;auto.
+      apply related_sts_pub_plus_priv_world;auto.
+      apply region_state_nwl_monotone_nm with W;auto.
+    - destruct l; auto. discriminate.
+    - iApply (big_sepL_mono with "Hw").
+      iIntros (n y Hsome) "Hw".
+      iDestruct "Hw" as (p Hfl) "#[Hrw Hrel ]".
+      iExists _. iSplit;eauto. iFrame "#".
+      iDestruct "Hrel" as %Hrel.
+      iPureIntro. destruct l; try discriminate.
+      apply region_state_nwl_monotone_nm_nl with W;auto.
+      apply related_sts_pub_plus_priv_world;auto.
+      apply region_state_nwl_monotone_nm with W;auto.
+    - iModIntro. iIntros (r W'').
+      destruct l; simpl; try discriminate.
+      + iIntros (Hrelated').
+        iAssert (future_world Global a W W'')%I as "Hrelated".
+        { iPureIntro. apply related_sts_pub_plus_priv_trans_world with W'; auto. }
+        iSpecialize ("Hw" $! r W'' with "Hrelated").
+        iApply "Hw".
+      + iIntros (Hrelated').
+        iAssert (future_world Local a W W'')%I as "Hrelated".
+        { iPureIntro. apply related_sts_pub_plus_trans_world with W'; auto. }
+        iSpecialize ("Hw" $! r W'' with "Hrelated").
+        iApply "Hw".
+    - iApply (big_sepL_mono with "Hw").
+      iIntros (n y Hsome) "Hw".
+      iDestruct "Hw" as (p Hfl) "#[Hrw Hrel ]".
+      iExists _. iSplit;eauto. iFrame "#".
+      iDestruct "Hrel" as %Hrel.
+      iPureIntro. destruct l; try discriminate.
+      apply region_state_nwl_monotone_nm_nl with W;auto.
+      apply related_sts_pub_plus_priv_world;auto.
+      apply region_state_nwl_monotone_nm with W;auto.
+    - destruct l; try discriminate. done. done.
+    - destruct l; simpl in Hnl; try discriminate.
+      + iApply (big_sepL_mono with "Hw").
+        iIntros (n y Hsome) "Hw".
+        iDestruct "Hw" as (p Hfl) "#[Hrw Hst ]".
+        iExists _. iSplit;eauto. iFrame "#".
+        iDestruct "Hst" as %Hst.
+        iPureIntro.
+        apply region_state_nwl_monotone_nm_nl with W;auto.
+        apply related_sts_pub_plus_priv_world;auto.
+      + iDestruct "Hw" as "[Hw1 Hw2]".
+        iSplit.
+        { iApply (big_sepL_mono with "Hw1").
+          iIntros (n y Hsome) "Hw".
+          iDestruct "Hw" as (p Hfl) "#[Hrw Hst ]".
+          iExists _. iSplit;eauto. iFrame "#".
+          iDestruct "Hst" as %Hst.
+          iPureIntro.
+          apply region_state_nwl_monotone_nm with W;auto. }
+        { iApply (big_sepL_mono with "Hw2").
+          iIntros (n y Hsome) "Hw".
+          iDestruct "Hw" as (p Hfl) "#[Hrw Hst ]".
+          iExists _. iSplit;eauto. iFrame "#".
+          iDestruct "Hst" as %Hst.
+          iPureIntro.
+          apply region_state_U_monotone with W;auto. }
+    - destruct l; auto. discriminate.
+    - destruct l; simpl in Hnl; try discriminate.
+      + iApply (big_sepL_mono with "Hw").
+        iIntros (n y Hsome) "Hw".
+        iDestruct "Hw" as (p Hfl) "#[Hrw Hst ]".
+        iExists _. iSplit;eauto. iFrame "#".
+        iDestruct "Hst" as %Hst.
+        iPureIntro.
+        apply region_state_nwl_monotone_nm_nl with W; auto.
+        apply related_sts_pub_plus_priv_world;auto.
+      + iDestruct "Hw" as "[Hw1 Hw2]".
+        iSplit.
+        { iApply (big_sepL_mono with "Hw1").
+          iIntros (n y Hsome) "Hw".
+          iDestruct "Hw" as (p Hfl) "#[Hrw Hst ]".
+          iExists _. iSplit;eauto. iFrame "#".
+          iDestruct "Hst" as %Hst.
+          iPureIntro.
+          apply region_state_nwl_monotone_nm with W;auto. }
+        { iApply (big_sepL_mono with "Hw2").
+          iIntros (n y Hsome) "Hw".
+          iDestruct "Hw" as (p Hfl) "#[Hrw Hst ]".
+          iExists _. iSplit;eauto. iFrame "#".
+          iDestruct "Hst" as %Hst.
+          iPureIntro.
+          apply region_state_U_monotone with W;auto. }
+    - destruct l; try discriminate. done. done.
+  Qed. 
+
+  Lemma interp_monotone_nm_nl W W' w :
     ⌜related_sts_priv_world W W'⌝ -∗ ⌜isLocalWord w = false⌝ -∗
     interp W w -∗ interp W' w.
   Proof.
@@ -283,14 +828,14 @@ Section monotone.
       iExists _. iSplit;eauto. iFrame "#".
       iDestruct "Hrel" as %Hrel.
       iPureIntro. destruct l; try discriminate.
-      apply region_state_nwl_monotone_nl with W;auto.
+      apply region_state_nwl_monotone_nm_nl with W;auto.
     - iApply (big_sepL_mono with "Hw").
       iIntros (n y Hsome) "Hw".
       iDestruct "Hw" as (p Hfl) "#[Hrw Hrel ]".
       iExists _. iSplit;eauto. iFrame "#".
       iDestruct "Hrel" as %Hrel.
       iPureIntro. destruct l; try discriminate.
-      apply region_state_nwl_monotone_nl with W;auto.
+      apply region_state_nwl_monotone_nm_nl with W;auto.
     - destruct l; auto. discriminate.
     - iApply (big_sepL_mono with "Hw").
       iIntros (n y Hsome) "Hw".
@@ -298,11 +843,11 @@ Section monotone.
       iExists _. iSplit;eauto. iFrame "#".
       iDestruct "Hrel" as %Hrel.
       iPureIntro. destruct l; try discriminate.
-      apply region_state_nwl_monotone_nl with W;auto.
+      apply region_state_nwl_monotone_nm_nl with W;auto.
     - iModIntro. iIntros (r W'').
       destruct l; simpl; try discriminate.
       iIntros (Hrelated').
-      iAssert (future_world Global W W'')%I as "Hrelated".
+      iAssert (future_world Global a0 W W'')%I as "Hrelated".
       { iPureIntro. apply related_sts_priv_trans_world with W'; auto. }
       iSpecialize ("Hw" $! r W'' with "Hrelated").
       iApply "Hw".
@@ -312,7 +857,7 @@ Section monotone.
       iExists _. iSplit;eauto. iFrame "#".
       iDestruct "Hrel" as %Hrel.
       iPureIntro. destruct l; try discriminate.
-      apply region_state_nwl_monotone_nl with W;auto.
+      apply region_state_nwl_monotone_nm_nl with W;auto.
     - destruct l; try discriminate. done.
     - destruct l; simpl in Hnl; try discriminate.
       iApply (big_sepL_mono with "Hw").
@@ -321,7 +866,7 @@ Section monotone.
       iExists _. iSplit;eauto. iFrame "#".
       iDestruct "Hst" as %Hst.
       iPureIntro.
-      apply region_state_nwl_monotone_nl with W; auto.
+      apply region_state_nwl_monotone_nm_nl with W; auto.
     - destruct l; auto. discriminate.
     - destruct l; simpl in Hnl; try discriminate.
       iApply (big_sepL_mono with "Hw").
@@ -330,32 +875,32 @@ Section monotone.
       iExists _. iSplit;eauto. iFrame "#".
       iDestruct "Hst" as %Hst.
       iPureIntro.
-      apply region_state_nwl_monotone_nl with W; auto.
+      apply region_state_nwl_monotone_nm_nl with W; auto.
     - destruct l; try discriminate. done.
   Qed.
 
   (*Lemma that allows switching between the two different formulations of monotonicity, to alleviate the effects of inconsistencies*)
-  Lemma switch_monotonicity_formulation ρ w p φ:
-      ρ ≠ Revoked → (∀ m, ρ ≠ Static m) ->
-      monotonicity_guarantees_region ρ w p φ ≡ monotonicity_guarantees_decide (Σ := Σ) ρ w p φ.
+  Lemma switch_monotonicity_formulation ρ l w p φ:
+      ρ ≠ Revoked → (∀ m, ρ ≠ Static m) -> (∀ m, ρ ≠ Monostatic m) -> (∀ w, ρ ≠ Uninitialized w) ->
+      monotonicity_guarantees_region ρ l w p φ ≡ monotonicity_guarantees_decide (Σ := Σ) ρ l w p φ.
   Proof.
-    intros Hrev Hsta. unfold monotonicity_guarantees_region, monotonicity_guarantees_decide.
+    intros Hrev Hsta Hmono Huninit.
+    unfold monotonicity_guarantees_region, monotonicity_guarantees_decide.
     iSplit; iIntros "HH".
-    - destruct ρ.
+    - destruct ρ;simpl;auto.
       * simpl. destruct (pwl p) ; intros.
         destruct (decide (Temporary = Temporary ∧ true = true)). auto. assert (Temporary = Temporary ∧ true = true); auto. by congruence.
         destruct (decide (Temporary = Temporary ∧ false = true)). destruct a; by exfalso. auto.
-      *  destruct (decide (Permanent = Temporary ∧ pwl p = true)). destruct a; by exfalso. auto.
+      * destruct (pwl p).
+        destruct (decide (Monotemporary = Monotemporary ∧ true = true)). auto. exfalso;auto.
+        simpl. auto.
       * by intros.
       * specialize (Hsta g). done.
-    - intros. destruct ρ.
-      * destruct (pwl p).
-        destruct (decide (Temporary = Temporary ∧ true = true)). auto.
-        assert (Temporary = Temporary ∧ true = true); auto. by congruence.
-        destruct (decide (Temporary = Temporary ∧ false = true)). destruct a; by exfalso. auto.
-      *  destruct (decide (Permanent = Temporary ∧ pwl p = true)). destruct a; by exfalso. auto.
-      * by iPureIntro.
-      * by iPureIntro.
+      * specialize (Hmono g). done.
+      * specialize (Huninit w0). done.
+    - intros. destruct ρ;simpl;auto.
+      * destruct (pwl p);simpl;auto.
+      * destruct (pwl p);simpl;auto.
   Qed.
 
   (* The validity of regions are monotone wrt private/public future worlds *)
@@ -372,62 +917,86 @@ Section monotone.
     iFrame.
     iDestruct "Hperm" as %Hperm.
     iPureIntro.
-    apply (region_state_nwl_monotone_nl _ W') in Hperm; auto.
+    apply (region_state_nwl_monotone_nm_nl _ W') in Hperm; auto.
   Qed.
 
   Lemma adv_stack_monotone W W' b e :
     related_sts_pub_world W W' ->
     ([∗ list] a ∈ region_addrs b e, read_write_cond a RWLX interp
-                                     ∧ ⌜region_state_pwl W a⌝)
+                                     ∧ ⌜region_state_pwl_mono W a⌝)
     -∗ ([∗ list] a ∈ region_addrs b e, read_write_cond a RWLX interp
-                                       ∧ ⌜region_state_pwl W' a⌝).
+                                       ∧ ⌜region_state_pwl_mono W' a⌝).
   Proof.
     iIntros (Hrelated) "Hstack_adv".
     iApply (big_sepL_mono with "Hstack_adv").
     iIntros (k y Hsome) "(Hr & Htemp)".
     iDestruct "Htemp" as %Htemp.
     iFrame. iPureIntro.
-    apply (region_state_pwl_monotone _ W') in Htemp; auto.
+    apply (region_state_pwl_monotone_mono _ W') in Htemp; auto.
   Qed.
 
-Global Instance interp_ne n :
-  Proper (dist n ==> dist n) (λ Wv : WORLD * (leibnizO Word), (interp Wv.1) Wv.2).
-Proof.
-  solve_proper.
-Qed.
-
-(*The general monotonicity statement that interp gives you when writing a word into a pointer (p0, l, a2, a1, a0) ; simply a bundling of all individual monotonicity statements*)
+  Global Instance interp_ne n :
+    Proper (dist n ==> dist n) (λ Wv : WORLD * (leibnizO Word), (interp Wv.1) Wv.2).
+  Proof.
+    solve_proper.
+  Qed.
+  
+  (* The general monotonicity statement that interp gives you when writing a word into a
+     pointer (p0, l, a2, a1, a0) ; simply a bundling of all individual monotonicity statements *)
 Lemma interp_monotone_generalW (W : WORLD)  (ρ : region_type) (p p0 p1 : Perm) (l g : Locality)(b e a a2 a1 a0 : Addr):
   std W !! a0 = Some ρ →
   withinBounds (p0, l, a2, a1, a0) = true →
   PermFlows p0 p1 →
-  (negb (isLocal g) || match p0 with
-                       | RWL | RWLX => true
-                       | _ => false
-                       end = true)→
+  canStore p0 a0 (inr (p,g,b,e,a)) = true →
   ((fixpoint interp1) W) (inr (p0, l, a2, a1, a0)) -∗
-  monotonicity_guarantees_region ρ  (inr (p, g, b, e, a)) p1  (λne Wv : WORLD * (leibnizO Word), (interp Wv.1) Wv.2).
+  monotonicity_guarantees_region ρ a0 (inr (p, g, b, e, a)) p1  (λne Wv : WORLD * (leibnizO Word), (interp Wv.1) Wv.2).
 Proof.
   unfold monotonicity_guarantees_region.
   iIntros (Hstd Hwb Hfl' Hconds) "#Hvdst".
-  destruct ρ.
-  - destruct (pwl p1) eqn: HpwlP1 ; iModIntro; simpl.
+  destruct ρ;auto.
+  - destruct (pwl p1) eqn: HpwlP1 ; iModIntro; simpl;auto.
     * iIntros (W0 W1) "% HIW0".
-        by iApply interp_monotone.
+      iApply (interp_monotone_nm with "[] [] HIW0");[done|].
+      destruct p0 ; try (simpl in Hconds; by exfalso).
+      all: destruct g;auto. 
+      all: iDestruct (writeLocalAllowed_valid_cap_implies with "Hvdst" ) as %Ha;eauto;rewrite Ha in Hstd;done.
     * iIntros (W0 W1) "% HIW0".
+      iApply (interp_monotone_nm_nl with "[] [] HIW0");[done|].
+      destruct g;auto.
+      ** destruct p0;inversion Hconds;destruct p1;inversion Hfl';done.
+      ** apply andb_prop in Hconds as [Hconds ?]. destruct p0;inversion Hconds;destruct p1;inversion Hfl';done.
+  - destruct (pwl p1) eqn: HpwlP1 ; iModIntro; simpl;auto.
+    + iIntros (W0 W1) "% HIW0".
       destruct g.
-    + by iApply interp_monotone_nl.
-    (*The below case is a contradiction, since if g is local,p0 must be WL and p0 flows into the non-WL p1*)
-    + destruct p0 ; try (simpl in Hconds; by exfalso).
-      all:destruct p1 eqn:Hp1v ; (by exfalso).
+      * iApply (interp_monotone_nm_nl with "[] [] HIW0");auto.
+        iPureIntro. apply related_sts_a_pub_plus_world in a3. apply related_sts_pub_plus_priv_world;auto. 
+      * iApply (interp_monotone_nm with "[] [] HIW0");auto.
+        iPureIntro. apply related_sts_a_pub_plus_world with a0;auto.
+      * destruct (decide (p = O)). 
+        { subst. rewrite !fixpoint_interp1_eq. done. }
+        iApply (interp_monotone_a with "[] HIW0");auto.
+        apply andb_prop in Hconds as [Hp0 Hleb].
+        simpl. destruct (isU p) eqn:Hu.
+        ** assert (a <= a0)%a as Hle.
+           { destruct p; inversion Hu;simpl in Hleb;apply Z.leb_le in Hleb;solve_addr. }
+           iPureIntro. apply related_sts_a_weak_world with a0;auto. 
+        ** assert (e <= a0)%a as Hle.
+           { destruct p; inversion Hu;simpl in Hleb;apply Z.leb_le in Hleb; try solve_addr. }
+           iPureIntro. apply related_sts_a_weak_world with a0;auto.
+    + assert (pwl p0 = false) as Hpwl.
+      { destruct p0;auto; destruct p1;inversion HpwlP1;inversion Hfl'. }
+      simpl in Hconds. rewrite Hpwl andb_false_l in Hconds. destruct g;inversion Hconds.
+      iIntros (W0 W1) "% HIW0".
+      iApply (interp_monotone_nm_nl with "[] [] HIW0");auto.
   - iModIntro. simpl. iIntros (W0 W1) "% HIW0".
     destruct g.
-    + by iApply interp_monotone_nl.
+    + by iApply interp_monotone_nm_nl.
     + (*Trick here: value relation leads to a contradiction if p0 is WL, since then its region cannot be permanent*)
       iDestruct ( writeLocalAllowed_valid_cap_implies with "Hvdst" ) as %Ha; eauto.
       rewrite Hstd in Ha. inversion Ha.
-  - auto.
-  - auto.
+    + apply andb_prop in Hconds as [Hp0 Hleb].
+      iDestruct ( writeLocalAllowed_valid_cap_implies with "Hvdst" ) as %Ha; eauto.
+      rewrite Hstd in Ha. inversion Ha.
 Qed.
 
 (* Analogous, but now we have the general monotonicity statement in case an integer z is written *)
@@ -436,20 +1005,19 @@ Lemma interp_monotone_generalZ (W : WORLD)  (ρ : region_type) (p0 p1 : Perm) (l
   withinBounds (p0, l, a2, a1, a0) = true →
   PermFlows p0 p1 →
   ((fixpoint interp1) W) (inr (p0, l, a2, a1, a0)) -∗
-  monotonicity_guarantees_region ρ  (inl z) p1  (λne Wv : WORLD * (leibnizO Word), (interp Wv.1) Wv.2).
+  monotonicity_guarantees_region ρ a0 (inl z) p1  (λne Wv : WORLD * (leibnizO Word), (interp Wv.1) Wv.2).
 Proof.
   unfold monotonicity_guarantees_region.
   iIntros (Hstd Hwb Hfl') "#Hvdst".
-  destruct ρ.
+  destruct ρ;auto.
   - destruct (pwl p1) eqn: HpwlP1 ; iModIntro; simpl.
-    * iIntros (W0 W1) "% HIW0".
-        by iApply interp_monotone.
-    * iIntros (W0 W1) "% HIW0".
-        by iApply interp_monotone_nl.
-  - iModIntro. simpl. iIntros (W0 W1) "% HIW0".
-      by iApply interp_monotone_nl.
-  - trivial.
-  - auto.
+    all: iIntros (W0 W1) "% HIW0".
+    all: rewrite !fixpoint_interp1_eq;done. 
+  - destruct (pwl p1) eqn: HpwlP1 ; iModIntro; simpl.
+    all: iIntros (W0 W1) "% HIW0".
+    all: rewrite !fixpoint_interp1_eq;done. 
+  - iModIntro. iIntros (W0 W1) "% HIW0".
+    iSimpl. rewrite !fixpoint_interp1_eq;done. 
 Qed.
 
 End monotone.
