theories/region_invariants_transitions.v
@@ -1,0 +1,498 @@
+From iris.proofmode Require Import tactics.
+From iris.program_logic Require Export weakestpre.
+From cap_machine Require Export region_invariants.
+From iris.base_logic Require Export invariants na_invariants saved_prop.
+Import uPred.
+
+
+Section transitions.
+  Context {Σ:gFunctors} {memg:memG Σ} {regg:regG Σ} 
+          {stsg : STSG Addr region_type Σ} {heapg : heapG Σ}
+          `{MonRef: MonRefG (leibnizO _) CapR_rtc Σ} 
+          `{MachineParameters}.
+
+  Implicit Types fsd gsd hsd : STS_std_states Addr region_type.
+  Notation STS := (leibnizO (STS_states * STS_rels)).
+  Notation STS_STD := (leibnizO (STS_std_states Addr region_type)).
+  Notation WORLD := (prodO STS_STD STS).
+  Implicit Types W : WORLD. 
+
+  (* --------------------------------------------------------------------------------- *)
+  (* --------------------- TRANSITIVITY LEMMA TO MOVE TO STS.V ----------------------- *)
+
+  Lemma related_sts_pub_pub_plus_trans fs fr gs gr hs hr :
+    related_sts_pub fs gs fr gr → related_sts_pub_plus gs hs gr hr →
+    related_sts_pub_plus fs hs fr hr.
+  Proof.
+    intros [Hf1 [Hf2 Hf3]] [Hg1 [Hg2 Hg3]]; split; [|split]; try by etrans.
+    intros i r1 r2 r1' r2' r3 r3' Hfr Hhr.
+    specialize (Hf1 i); specialize (Hf2 i);
+      revert Hf1 Hf2; rewrite !elem_of_dom; intros Hf1 Hf2.
+    destruct Hf2; eauto. destruct x as [[x1 x2] x3].
+    edestruct Hf3 as [Heq1 [Heq2 [Heq3 Hrtc]] ] ; eauto; simplify_eq.
+    edestruct Hg3 as [Heq1 [Heq2 [Heq3 Hrtc']] ] ; eauto; simplify_eq.
+    repeat (split;auto).
+    intros x y Hx Hy.
+    destruct Hf1;eauto.
+    etrans;eauto.
+    apply rtc_or_intro; auto.
+  Qed.
+
+  Lemma related_sts_std_pub_pub_plus_trans fsd gsd hsd :
+    related_sts_std_pub fsd gsd → related_sts_std_pub_plus gsd hsd →
+    related_sts_std_pub_plus fsd hsd.
+  Proof.
+    intros [Hf1 Hf2] [Hg1 Hg2]; split; try by etrans.
+    intros i x y Hx Hy.
+    specialize (Hf1 i);
+      revert Hf1; rewrite !elem_of_dom; intros Hf1.
+    destruct Hf1 as [x0 Hx0]; eauto.
+    specialize (Hf2 i x x0 Hx Hx0); simplify_eq.
+    specialize (Hg2 i x0 y Hx0 Hy); simplify_eq.
+    etrans;eauto.
+    apply rtc_or_intro; auto.
+  Qed.
+
+  Lemma related_sts_pub_pub_plus_trans_world W W' W'' :
+    related_sts_pub_world W W' → related_sts_pub_plus_world W' W''
+    → related_sts_pub_plus_world W W''.
+  Proof.
+    intros [Hrel Hrel'] [Hrel2 Hrel2'].
+    split.
+    - apply related_sts_std_pub_pub_plus_trans with W'.1;auto.
+    - apply related_sts_pub_pub_plus_trans with W'.2.1 W'.2.2;auto.
+  Qed.
+
+  Lemma related_sts_std_pub_a_trans a fsd gsd hsd :
+    related_sts_std_pub fsd gsd → related_sts_a gsd hsd a →
+    related_sts_a fsd hsd a.
+  Proof.
+    intros [Hf1 Hf2] [Hg1 Hg2]; split; try by etrans.
+    intros i x y Hx Hy.
+    specialize (Hf1 i);
+      revert Hf1; rewrite !elem_of_dom; intros Hf1.
+    destruct Hf1 as [x0 Hx0]; eauto.
+    specialize (Hf2 i x x0 Hx Hx0); simplify_eq.
+    specialize (Hg2 i x0 y Hx0 Hy); simplify_eq.
+    etrans;eauto. eapply rtc_implies;eauto.
+    intros r q Hr. destruct (decide (le_a i a));auto.
+  Qed.
+
+  Lemma related_sts_std_a_pub_plus_trans a fsd gsd hsd :
+    related_sts_a fsd gsd a → related_sts_std_pub_plus gsd hsd →
+    related_sts_std_pub_plus fsd hsd.
+  Proof.
+    intros [Hf1 Hf2] [Hg1 Hg2]; split; try by etrans.
+    intros i x y Hx Hy.
+    specialize (Hf1 i);
+      revert Hf1; rewrite !elem_of_dom; intros Hf1.
+    destruct Hf1 as [x0 Hx0]; eauto.
+    specialize (Hf2 i x x0 Hx Hx0); simplify_eq.
+    specialize (Hg2 i x0 y Hx0 Hy); simplify_eq.
+    etrans;eauto. eapply rtc_implies;[|apply Hf2].
+    intros r q Hr. destruct (decide (le_a i a));auto.
+  Qed.
+
+  Lemma related_sts_std_a_priv_trans a fsd gsd hsd :
+    related_sts_a fsd gsd a → related_sts_std_priv gsd hsd →
+    related_sts_std_priv fsd hsd.
+  Proof.
+    intros [Hf1 Hf2] [Hg1 Hg2]; split; try by etrans.
+    intros i x y Hx Hy.
+    specialize (Hf1 i);
+      revert Hf1; rewrite !elem_of_dom; intros Hf1.
+    destruct Hf1 as [x0 Hx0]; eauto.
+    specialize (Hf2 i x x0 Hx Hx0); simplify_eq.
+    specialize (Hg2 i x0 y Hx0 Hy); simplify_eq.
+    etrans;eauto. eapply rtc_implies;[|apply Hf2].
+    intros r q. destruct (decide (le_a i a));auto.
+    intros [? | ?];auto. 
+  Qed.
+
+  Lemma related_sts_std_pub_plus_priv_trans fsd gsd hsd :
+    related_sts_std_pub_plus fsd gsd → related_sts_std_priv gsd hsd →
+    related_sts_std_priv fsd hsd.
+  Proof.
+    intros [Hf1 Hf2] [Hg1 Hg2]; split; try by etrans.
+    intros i x y Hx Hy.
+    specialize (Hf1 i);
+      revert Hf1; rewrite !elem_of_dom; intros Hf1.
+    destruct Hf1 as [x0 Hx0]; eauto.
+    specialize (Hf2 i x x0 Hx Hx0); simplify_eq.
+    specialize (Hg2 i x0 y Hx0 Hy); simplify_eq.
+    etrans;eauto. eapply rtc_implies;[|apply Hf2].
+    intros r q. intros [? | ?];auto.
+  Qed.
+
+  Lemma related_sts_std_pub_plus_trans fsd gsd hsd :
+    related_sts_std_pub_plus fsd gsd → related_sts_std_pub_plus gsd hsd →
+    related_sts_std_pub_plus fsd hsd.
+  Proof.
+    intros [Hf1 Hf2] [Hg1 Hg2]; split; try by etrans.
+    intros i x y Hx Hy.
+    specialize (Hf1 i);
+      revert Hf1; rewrite !elem_of_dom; intros Hf1.
+    destruct Hf1 as [x0 Hx0]; eauto.
+    specialize (Hf2 i x x0 Hx Hx0); simplify_eq.
+    specialize (Hg2 i x0 y Hx0 Hy); simplify_eq.
+    etrans;eauto. 
+  Qed.
+
+  Lemma related_sts_pub_plus_trans fs fr gs gr hs hr :
+    related_sts_pub_plus fs gs fr gr → related_sts_pub_plus gs hs gr hr →
+    related_sts_pub_plus fs hs fr hr.
+  Proof.
+    intros [Hf1 [Hf2 Hf3]] [Hg1 [Hg2 Hg3]]; split; [|split]; try by etrans.
+    intros i r1 r2 r1' r2' r3 r3' Hfr Hhr.
+    specialize (Hf1 i); specialize (Hf2 i);
+      revert Hf1 Hf2; rewrite !elem_of_dom; intros Hf1 Hf2.
+    destruct Hf2; eauto. destruct x as [[x1 x2] x3].
+    edestruct Hf3 as [Heq1 [Heq2 [Heq3 Hrtc]] ] ; eauto; simplify_eq.
+    edestruct Hg3 as [Heq1 [Heq2 [Heq3 Hrtc']] ] ; eauto; simplify_eq.
+    repeat (split;auto).
+    intros x y Hx Hy.
+    destruct Hf1;eauto.
+    etrans;eauto.
+  Qed.
+
+  Lemma related_sts_pub_plus_priv_trans fs fr gs gr hs hr :
+    related_sts_pub_plus fs gs fr gr → related_sts_priv gs hs gr hr →
+    related_sts_priv fs hs fr hr.
+  Proof.
+    intros [Hf1 [Hf2 Hf3]] [Hg1 [Hg2 Hg3]]; split; [|split]; try by etrans.
+    intros i r1 r2 r1' r2' r3 r3' Hfr Hhr.
+    specialize (Hf1 i); specialize (Hf2 i);
+      revert Hf1 Hf2; rewrite !elem_of_dom; intros Hf1 Hf2.
+    destruct Hf2; eauto. destruct x as [[x1 x2] x3].
+    edestruct Hf3 as [Heq1 [Heq2 [Heq3 Hrtc]] ] ; eauto; simplify_eq.
+    edestruct Hg3 as [Heq1 [Heq2 [Heq3 Hrtc']] ] ; eauto; simplify_eq.
+    repeat (split;auto).
+    intros x y Hx Hy.
+    destruct Hf1;eauto.
+    etrans;eauto. eapply rtc_implies;[|apply Hrtc];auto.
+    intros r q [Hr | Hr];auto. 
+  Qed.
+
+  Lemma related_sts_pub_a_trans_world W W' W'' a :
+    related_sts_pub_world W W' → related_sts_a_world W' W'' a
+    → related_sts_a_world W W'' a.
+  Proof.
+    intros [Hrel Hrel'] [Hrel2 Hrel2'].
+    split.
+    - apply related_sts_std_pub_a_trans with W'.1;auto.
+    - apply related_sts_pub_pub_plus_trans with W'.2.1 W'.2.2;auto.
+  Qed.
+
+  Lemma related_sts_a_pub_plus_trans_world W W' W'' a :
+    related_sts_a_world W W' a → related_sts_pub_plus_world W' W''
+    → related_sts_pub_plus_world W W''.
+  Proof.
+    intros [Hrel Hrel'] [Hrel2 Hrel2'].
+    split.
+    - apply related_sts_std_a_pub_plus_trans with a W'.1;auto.
+    - apply related_sts_pub_plus_trans with W'.2.1 W'.2.2;auto.
+  Qed.
+
+  Lemma related_sts_a_priv_trans_world W W' W'' a :
+    related_sts_a_world W W' a → related_sts_priv_world W' W''
+    → related_sts_priv_world W W''.
+  Proof.
+    intros [Hrel Hrel'] [Hrel2 Hrel2'].
+    split.
+    - apply related_sts_std_a_priv_trans with a W'.1;auto.
+    - apply related_sts_pub_plus_priv_trans with W'.2.1 W'.2.2;auto.
+  Qed.
+
+  Lemma related_sts_a_trans_world W W' W'' a :
+    related_sts_a_world W W' a → related_sts_a_world W' W'' a →
+    related_sts_a_world W W'' a.
+  Proof.
+    intros [Hrel Hrel'] [Hrel2 Hrel2'].
+    split.
+    - apply related_sts_a_trans_left with W'.1 a;auto. done.
+    - apply related_sts_pub_plus_trans with W'.2.1 W'.2.2;auto.
+  Qed.
+
+
+  Lemma related_sts_pub_plus_priv_trans_world W W' W'' :
+    related_sts_pub_plus_world W W' → related_sts_priv_world W' W'' →
+    related_sts_priv_world W W''.
+  Proof.
+    intros [Hrel Hrel'] [Hrel2 Hrel2'].
+    split.
+    - apply related_sts_std_pub_plus_priv_trans with W'.1;auto.
+    - apply related_sts_pub_plus_priv_trans with W'.2.1 W'.2.2;auto.
+  Qed.
+
+  Lemma related_sts_pub_plus_trans_world W W' W'' :
+    related_sts_pub_plus_world W W' → related_sts_pub_plus_world W' W'' →
+    related_sts_pub_plus_world W W''.
+  Proof.
+    intros [Hrel Hrel'] [Hrel2 Hrel2'].
+    split.
+    - apply related_sts_std_pub_plus_trans with W'.1;auto.
+    - apply related_sts_pub_plus_trans with W'.2.1 W'.2.2;auto.
+  Qed.
+
+
+  (* --------------------------------------------------------------------------------- *)
+  (* ------------------------- LEMMAS ABOUT STD TRANSITIONS -------------------------- *)
+
+  Lemma std_rel_pub_Permanent x :
+    std_rel_pub Permanent x → x = Permanent.
+  Proof.
+    intros Hrel.
+    inversion Hrel.
+  Qed.
+
+  Lemma std_rel_pub_rtc_Permanent x y :
+    x = Permanent →
+    rtc std_rel_pub x y → y = Permanent.
+  Proof.
+    intros Hx Hrtc.
+    induction Hrtc;auto.
+    subst. apply IHHrtc. apply std_rel_pub_Permanent; auto.
+  Qed.
+
+  Lemma std_rel_pub_plus_Permanent x :
+    std_rel_pub_plus Permanent x → x = Permanent.
+  Proof.
+    intros Hrel.
+    inversion Hrel.
+  Qed.
+
+  Lemma std_rel_pub_plus_rtc_Permanent x y :
+    x = Permanent →
+    rtc (λ x y : region_type, std_rel_pub x y ∨ std_rel_pub_plus x y) x y →
+    y = Permanent.
+  Proof.
+    intros Hx Hrtc.
+    induction Hrtc as [|x y z Hrel];auto.
+    subst. destruct Hrel as [Hpub | Hpubp]. 
+    - apply std_rel_pub_Permanent in Hpub. auto.
+    - apply std_rel_pub_plus_Permanent in Hpubp. auto.
+  Qed.
+
+  Lemma std_rel_priv_Permanent x :
+    std_rel_priv Permanent x → x = Permanent.
+  Proof.
+    intros Hrel.
+    inversion Hrel; done.
+  Qed.
+
+  Lemma std_rel_priv_rtc_Permanent x y :
+    x = Permanent →
+    rtc std_rel_priv x y → y = Permanent.
+  Proof.
+    intros Hx Hrtc.
+    induction Hrtc;auto.
+    subst. apply IHHrtc. apply std_rel_priv_Permanent; auto.
+  Qed.
+
+  Lemma std_rel_rtc_Permanent x y :
+    x = Permanent →
+    rtc (λ x0 y0 : region_type, std_rel_pub x0 y0 ∨ std_rel_pub_plus x0 y0 ∨ std_rel_priv x0 y0) x y →
+    y = Permanent.
+  Proof.
+    intros Hx Hrtc.
+    induction Hrtc as [|x y z Hrel];auto.
+    subst. destruct Hrel as [Hrel | [Hrel | Hrel] ].
+    - apply std_rel_pub_Permanent in Hrel. auto.
+    - apply std_rel_pub_plus_Permanent in Hrel. auto.
+    - apply std_rel_priv_Permanent in Hrel. auto.
+  Qed.
+
+  Lemma std_rel_pub_Temporary x :
+    std_rel_pub Temporary x → x = Temporary.
+  Proof.
+    intros Hrel.
+    inversion Hrel.
+  Qed.
+
+  Lemma std_rel_pub_plus_Temporary x :
+    std_rel_pub_plus Temporary x → x = Temporary.
+  Proof.
+    intros Hrel.
+    inversion Hrel.
+  Qed.
+
+  Lemma std_rel_pub_plus_rtc_Temporary x y :
+    x = Temporary →
+    rtc (λ x0 y0 : region_type, std_rel_pub x0 y0 ∨ std_rel_pub_plus x0 y0) x y → y = Temporary.
+  Proof.
+    intros Hx Hrtc.
+    induction Hrtc ;auto.
+    subst. destruct H0 as [Hrel | Hrel].
+    - apply IHHrtc. apply std_rel_pub_Temporary; auto.
+    - apply IHHrtc. apply std_rel_pub_plus_Temporary; auto.
+  Qed.
+
+  Lemma std_rel_pub_rtc_Temporary x y :
+    x = Temporary →
+    rtc std_rel_pub x y → y = Temporary.
+  Proof.
+    intros Hx Hrtc.
+    induction Hrtc ;auto.
+    subst. apply IHHrtc. apply std_rel_pub_Temporary; auto.
+  Qed.
+
+  Lemma std_rel_pub_Monotemporary x :
+    std_rel_pub Monotemporary x → x = Monotemporary.
+  Proof.
+    intros Hrel.
+    inversion Hrel.
+  Qed.
+
+  Lemma std_rel_pub_rtc_Monotemporary x y :
+    x = Monotemporary →
+    rtc std_rel_pub x y → y = Monotemporary.
+  Proof.
+    intros Hx Hrtc.
+    induction Hrtc ;auto.
+    subst. apply IHHrtc. apply std_rel_pub_Monotemporary; auto.
+  Qed.
+
+  Lemma std_rel_pub_Revoked x :
+    std_rel_pub Revoked x → x = Temporary ∨ x = Permanent ∨ x = Monotemporary.
+  Proof.
+    intros Hrel.
+    inversion Hrel; auto.
+  Qed.
+
+  Lemma std_rel_pub_rtc_Revoked x y :
+    x = Revoked →
+    rtc std_rel_pub x y → y = Temporary ∨ y = Permanent ∨ y = Monotemporary ∨ y = Revoked.
+  Proof.
+    intros Hx Hrtc.
+    inversion Hrtc; subst; auto.
+    apply std_rel_pub_Revoked in H0 as [-> | [-> | ->] ];auto. 
+    - left. eapply std_rel_pub_rtc_Temporary;eauto.
+    - right. left. eapply std_rel_pub_rtc_Permanent;eauto.
+    - right. right. left. eapply std_rel_pub_rtc_Monotemporary;eauto.
+  Qed.
+  
+  Lemma std_rel_pub_Static x g :
+    std_rel_pub (Static g) x → x = Temporary.
+  Proof.
+    intros Hrel.
+    inversion Hrel. auto. 
+  Qed.
+
+  Lemma std_rel_pub_plus_Static x g :
+    std_rel_pub_plus (Static g) x → x = Temporary.
+  Proof.
+    intros Hrel.
+    inversion Hrel. 
+  Qed.
+
+  Lemma std_rel_pub_Monostatic x g :
+    std_rel_pub (Monostatic g) x → x = Monotemporary.
+  Proof.
+    intros Hrel.
+    inversion Hrel. auto. 
+  Qed.
+
+  Lemma std_rel_pub_Uninitialized x w :
+    std_rel_pub (Uninitialized w) x → x = Monotemporary.
+  Proof.
+    intros Hrel.
+    inversion Hrel. auto. 
+  Qed.
+
+  Lemma std_rel_pub_rtc_Static x y g :
+    x = (Static g) →
+    rtc std_rel_pub x y → y = Temporary ∨ y = (Static g).
+  Proof.
+    intros Hx Hrtc.
+    inversion Hrtc; subst; auto. left.
+    apply std_rel_pub_Static in H0. 
+    eapply std_rel_pub_rtc_Temporary;eauto.
+  Qed.
+
+  Lemma std_rel_pub_rtc_Uninitialized x y w :
+    x = (Uninitialized w) →
+    rtc std_rel_pub x y → y = Monotemporary ∨ y = (Uninitialized w).
+  Proof.
+    intros Hx Hrtc.
+    inversion Hrtc; subst; auto. left.
+    apply std_rel_pub_Uninitialized in H0. 
+    eapply std_rel_pub_rtc_Monotemporary;eauto.
+  Qed.
+
+  Lemma std_rel_pub_plus_rtc_Static x y g :
+    x = (Static g) →
+    rtc (λ x0 y0, std_rel_pub x0 y0 ∨ std_rel_pub_plus x0 y0) x y → y = Temporary ∨ y = (Static g).
+  Proof.
+    intros Hx Hrtc.
+    induction Hrtc ;auto.
+    subst. destruct H0 as [Hrel | Hrel].
+    - apply std_rel_pub_Static in Hrel; auto. subst. 
+      eapply std_rel_pub_plus_rtc_Temporary in Hrtc;eauto.
+    - apply std_rel_pub_plus_Static in Hrel; auto. subst.
+      eapply std_rel_pub_plus_rtc_Temporary in Hrtc;eauto.
+  Qed.
+
+  Lemma std_rel_pub_rtc_Monostatic x y g :
+    x = (Monostatic g) →
+    rtc std_rel_pub x y → y = Monotemporary ∨ y = (Monostatic g).
+  Proof.
+    intros Hx Hrtc.
+    inversion Hrtc; subst; auto. left.
+    apply std_rel_pub_Monostatic in H0. 
+    eapply std_rel_pub_rtc_Monotemporary;eauto.
+  Qed.
+
+  Lemma std_rel_pub_plus_Monostatic x g :
+    std_rel_pub_plus (Monostatic g) x → x = (Monostatic g).
+  Proof.
+    intros Hrel; inversion Hrel. Qed.
+
+  Lemma std_rel_pub_plus_Uninitialized x w :
+    std_rel_pub_plus (Uninitialized w) x → x = (Uninitialized w).
+  Proof.
+    intros Hrel; inversion Hrel. Qed.
+
+  Lemma std_rel_pub_plus_Monotemporary x :
+    std_rel_pub_plus Monotemporary x → ∃ w, x = Uninitialized w.
+  Proof.
+    intros Hrel. inversion Hrel. eauto. Qed. 
+
+  Lemma std_rel_pub_plus_rtc_Monotemporary_or_Uninitialized x y :
+    x = Monotemporary ∨ (∃ w, x = Uninitialized w) →
+    rtc (λ x0 y0, std_rel_pub x0 y0 ∨ std_rel_pub_plus x0 y0) x y →
+    y = Monotemporary ∨ ∃ w, y = Uninitialized w.
+  Proof.
+    intros Hx Hrtc.
+    induction Hrtc ;[destruct Hx;eauto|].
+    destruct Hx as [-> | [g ->] ].
+    - destruct H0 as [Hpub | Hpubp]. 
+      + apply std_rel_pub_Monotemporary in Hpub. auto. 
+      + apply std_rel_pub_plus_Monotemporary in Hpubp as [g' ->].
+        apply IHHrtc. eauto. 
+    - destruct H0 as [Hpub | Hpubp]. 
+      + apply std_rel_pub_Uninitialized in Hpub. auto. 
+      + apply std_rel_pub_plus_Uninitialized in Hpubp as ->.
+        apply IHHrtc. eauto. 
+  Qed. 
+
+  Lemma std_rel_pub_plus_rtc_Uninitialized x y w :
+    x = Uninitialized w →
+    rtc (λ x0 y0, std_rel_pub x0 y0 ∨ std_rel_pub_plus x0 y0) x y →
+    y = Monotemporary ∨ (∃ w', y = Uninitialized w').
+  Proof.
+    intros Hx Hrtc.
+    eapply std_rel_pub_plus_rtc_Monotemporary_or_Uninitialized;eauto. 
+  Qed. 
+
+  Lemma std_rel_pub_plus_rtc_Monotemporary x y :
+    x = Monotemporary →
+    rtc (λ x0 y0, std_rel_pub x0 y0 ∨ std_rel_pub_plus x0 y0) x y →
+    y = Monotemporary ∨ ∃ w, y = Uninitialized w.
+  Proof.
+    intros Hx Hrtc. subst. 
+    apply (std_rel_pub_plus_rtc_Monotemporary_or_Uninitialized Monotemporary);eauto. 
+  Qed. 
+
+End transitions.
+
+
